GroupoidModel/Russell_PER_MS/Inversion.lean
@@ -9,12 +9,12 @@ open SubstProof
 
 /-! ## Context conversion -/
 
-theorem IndWfSb.conv_binder {Γ A A' l} : WfCtx Γ → Γ ⊢[l] A → Γ ⊢[l] A' → Γ ⊢[l] A ≡ A' →
-    IndWfSb ((A', l) :: Γ) Expr.bvar ((A, l) :: Γ) := by
+theorem wfSb_conv_binder {Γ A A' l} : WfCtx Γ → Γ ⊢[l] A → Γ ⊢[l] A' → Γ ⊢[l] A ≡ A' →
+    WfSb ((A', l) :: Γ) Expr.bvar ((A, l) :: Γ) := by
   intro Γ A A' AA'
   rw [show Expr.bvar = Expr.up Expr.bvar by autosubst, Expr.up_eq_snoc]
-  apply IndWfSb.snoc
-  . apply IndWfSb.wk <;> assumption
+  apply wfSb_snoc
+  . apply wfSb_wk <;> assumption
   . convert rename_all.2.1 A (WfCtx.snoc Γ A') (@WfRen.wk _ _ _) using 1; autosubst
   . apply WfTm.conv (WfTm.bvar (WfCtx.snoc Γ A') (Lookup.zero ..))
     convert rename_all.2.2.1 AA'.symm_tp (WfCtx.snoc Γ A') (@WfRen.wk _ _ _) using 1 <;> autosubst
@@ -22,13 +22,13 @@ theorem IndWfSb.conv_binder {Γ A A' l} : WfCtx Γ → Γ ⊢[l] A → Γ ⊢[l]
 theorem tp_conv_binder {Γ A A' B l l'} : WfCtx Γ → Γ ⊢[l] A → Γ ⊢[l] A' → Γ ⊢[l] A ≡ A' →
     (A, l) :: Γ ⊢[l'] B → (A', l) :: Γ ⊢[l'] B := by
   intro Γ A A' AA' B
-  convert (subst_all.2.1 B (WfCtx.snoc Γ A') (IndWfSb.conv_binder Γ A A' AA')).1 using 1
+  convert (subst_all.2.1 B (WfCtx.snoc Γ A') (wfSb_conv_binder Γ A A' AA')).1 using 1
   autosubst
 
 theorem tm_conv_binder {Γ A A' B t l l'} : WfCtx Γ → Γ ⊢[l] A → Γ ⊢[l] A' → Γ ⊢[l] A ≡ A' →
     (A, l) :: Γ ⊢[l'] t : B → (A', l) :: Γ ⊢[l'] t : B := by
   intro Γ A A' AA' t
-  convert (subst_all.2.2.2.1 t (WfCtx.snoc Γ A') (IndWfSb.conv_binder Γ A A' AA')).1 using 1 <;>
+  convert (subst_all.2.2.2.1 t (WfCtx.snoc Γ A') (wfSb_conv_binder Γ A A' AA')).1 using 1 <;>
     autosubst
 
 /-! ## Weakening -/
@@ -49,14 +49,14 @@ theorem tm_wk {Γ A B b l l'} : WfCtx Γ → Γ ⊢[l] A → Γ ⊢[l'] b : B �
 theorem tp_inst {Γ A B t l l'} : WfCtx Γ → Γ ⊢[l] A → Γ ⊢[l] t : A → (A, l) :: Γ ⊢[l'] B →
     Γ ⊢[l'] B.subst t.toSb :=
   fun Γ A t B =>
-    subst_all.2.1 B Γ (IndWfSb.snoc (IndWfSb.id Γ)
+    subst_all.2.1 B Γ (wfSb_snoc (WfSb.id Γ)
       (by convert A; autosubst) (by convert t; autosubst)) |>.1
 
 theorem tm_inst {Γ A B b t l l'} : WfCtx Γ → Γ ⊢[l] A → Γ ⊢[l] t : A →
     (A, l) :: Γ ⊢[l'] b : B →
     Γ ⊢[l'] b.subst t.toSb : B.subst t.toSb :=
   fun Γ A t b =>
-    subst_all.2.2.2.1 b Γ (IndWfSb.snoc (IndWfSb.id Γ)
+    subst_all.2.2.2.1 b Γ (wfSb_snoc (WfSb.id Γ)
       (by convert A; autosubst) (by convert t; autosubst)) |>.1
 
 theorem eqtp_inst {Γ A B B' t t' l l'} : WfCtx Γ → Γ ⊢[l] A →
@@ -64,8 +64,8 @@ theorem eqtp_inst {Γ A B B' t t' l l'} : WfCtx Γ → Γ ⊢[l] A →
     ((A, l) :: Γ) ⊢[l'] B ≡ B' →
     Γ ⊢[l'] B.subst t.toSb ≡ B'.subst t'.toSb := by
   intro Γ A t t' tt' BB'
-  apply subst_all.2.2.1 BB' Γ (IndWfSb.snoc _ _ _) (IndWfSb.snoc _ _ _) (IndEqSb.snoc _ _ _ _ _)
-  all_goals (try autosubst); grind [IndWfSb.id, IndEqSb.refl, EqTp.refl_tp]
+  apply subst_all.2.2.1 BB' Γ (wfSb_snoc _ _ _) (wfSb_snoc _ _ _) (eqSb_snoc _ _ _ _ _)
+  all_goals (try autosubst); grind [WfSb.id, EqSb.refl, EqTp.refl_tp]
 
 attribute [local grind] tp_conv_binder tm_conv_binder in
 theorem inv_all :
@@ -134,8 +134,8 @@ theorem inv_all :
       . apply (subst_all.2.1 Bwf _ _).1
         . grind [tp_wk, WfCtx.snoc]
         . rw [Expr.up_eq_snoc]
-          apply IndWfSb.snoc
-          . apply IndWfSb.ofRen
+          apply wfSb_snoc
+          . apply WfSb.ofRen
             . grind [tp_wk, WfCtx.snoc]
             . apply @WfRen.comp _ _ _ _ _ (@WfRen.wk _ _ _) (@WfRen.wk _ _ _)
           . convert tp_wk (B := A.subst Expr.wk) _ _ _ using 1
@@ -176,28 +176,48 @@ theorem WfCtx.snoc_inv {Γ A l} : WfCtx ((A, l) :: Γ) → Γ ⊢[l] A
 
 /-! ## Type former inversion -/
 
-theorem WfTp.inv_pi {Γ A B l l'} : Γ ⊢[max l l'] .pi l l' A B →
-    (Γ ⊢[l] A) ∧ ((A,l) :: Γ ⊢[l'] B) := by
+theorem WfTp.inv_pi {Γ A B l₀ l l'} : Γ ⊢[l₀] .pi l l' A B →
+    l₀ = max l l' ∧ (Γ ⊢[l] A) ∧ ((A,l) :: Γ ⊢[l'] B) := by
   suffices
       (∀ {Γ}, WfCtx Γ → True) ∧
-      (∀ {Γ l A}, Γ ⊢[l] A → ∀ {A' B l₁ l₂}, l = max l₁ l₂ → A = .pi l₁ l₂ A' B →
-        (Γ ⊢[l₁] A') ∧ ((A', l₁) :: Γ ⊢[l₂] B)) ∧
+      (∀ {Γ l A}, Γ ⊢[l] A → ∀ {A' B l₁ l₂}, A = .pi l₁ l₂ A' B →
+        l = max l₁ l₂ ∧ (Γ ⊢[l₁] A') ∧ ((A', l₁) :: Γ ⊢[l₂] B)) ∧
       (∀ {Γ l A B}, Γ ⊢[l] A ≡ B → True) ∧
       (∀ {Γ l t C}, Γ ⊢[l] t : C → True) ∧
       (∀ {Γ l t u A}, Γ ⊢[l] t ≡ u : A → True) from
-    fun h => this.2.1 h rfl rfl
+    fun h => this.2.1 h rfl
   mutual_induction <;> grind
 
-theorem WfTp.inv_sigma {Γ A B l l'} : Γ ⊢[max l l'] .sigma l l' A B →
-    (Γ ⊢[l] A) ∧ ((A,l) :: Γ ⊢[l'] B) := by
+theorem WfTp.inv_sigma {Γ A B l₀ l l'} : Γ ⊢[l₀] .sigma l l' A B →
+    l₀ = max l l' ∧ (Γ ⊢[l] A) ∧ ((A,l) :: Γ ⊢[l'] B) := by
   suffices
       (∀ {Γ}, WfCtx Γ → True) ∧
-      (∀ {Γ l A}, Γ ⊢[l] A → ∀ {A' B l₁ l₂}, l = max l₁ l₂ → A = .sigma l₁ l₂ A' B →
-        (Γ ⊢[l₁] A') ∧ ((A', l₁) :: Γ ⊢[l₂] B)) ∧
+      (∀ {Γ l A}, Γ ⊢[l] A → ∀ {A' B l₁ l₂}, A = .sigma l₁ l₂ A' B →
+        l = max l₁ l₂ ∧ (Γ ⊢[l₁] A') ∧ ((A', l₁) :: Γ ⊢[l₂] B)) ∧
       (∀ {Γ l A B}, Γ ⊢[l] A ≡ B → True) ∧
       (∀ {Γ l t C}, Γ ⊢[l] t : C → True) ∧
       (∀ {Γ l t u A}, Γ ⊢[l] t ≡ u : A → True) from
-    fun h => this.2.1 h rfl rfl
+    fun h => this.2.1 h rfl
+  mutual_induction <;> grind
+
+theorem WfTp.inv_univ {Γ l₀ l} : Γ ⊢[l₀] .univ l → l₀ = l+1 := by
+  suffices
+      (∀ {Γ}, WfCtx Γ → True) ∧
+      (∀ {Γ l A}, Γ ⊢[l] A → ∀ {l₁}, A = .univ l₁ → l = l₁+1) ∧
+      (∀ {Γ l A B}, Γ ⊢[l] A ≡ B → True) ∧
+      (∀ {Γ l t C}, Γ ⊢[l] t : C → True) ∧
+      (∀ {Γ l t u A}, Γ ⊢[l] t ≡ u : A → True) from
+    fun h => this.2.1 h rfl
+  mutual_induction <;> grind
+
+theorem WfTp.inv_el {Γ a l} : Γ ⊢[l] .el a → Γ ⊢[l+1] a : .univ l := by
+  suffices
+      (∀ {Γ}, WfCtx Γ → True) ∧
+      (∀ {Γ l A}, Γ ⊢[l] A → ∀ {a}, A = .el a → Γ ⊢[l+1] a : .univ l) ∧
+      (∀ {Γ l A B}, Γ ⊢[l] A ≡ B → True) ∧
+      (∀ {Γ l t C}, Γ ⊢[l] t : C → True) ∧
+      (∀ {Γ l t u A}, Γ ⊢[l] t ≡ u : A → True) from
+    fun h => this.2.1 h rfl
   mutual_induction <;> grind
 
 /-! ## Smart constructors -/
@@ -234,7 +254,7 @@ theorem WfTm.app {Γ A B f a l l'} :
     Γ ⊢[l] a : A →
     Γ ⊢[l'] .app l l' B f a : B.subst a.toSb :=
   fun hf ha =>
-    have ⟨hA, hB⟩ := hf.wf_tp.inv_pi
+    have ⟨_, hA, hB⟩ := hf.wf_tp.inv_pi
     WfTm.app' hA hB hf ha
 
 theorem WfTm.pair {Γ A B t u l l'} :
@@ -248,14 +268,14 @@ theorem WfTm.fst {Γ A B p l l'} :
     Γ ⊢[max l l'] p : .sigma l l' A B →
     Γ ⊢[l] .fst l l' A B p : A :=
   fun hp =>
-    have ⟨hA, hB⟩ := hp.wf_tp.inv_sigma
+    have ⟨_, hA, hB⟩ := hp.wf_tp.inv_sigma
     WfTm.fst' hA hB hp
 
 theorem WfTm.snd {Γ A B p l l'} :
     Γ ⊢[max l l'] p : .sigma l l' A B →
     Γ ⊢[l'] .snd l l' A B p : B.subst (Expr.fst l l' A B p).toSb :=
   fun hp =>
-    have ⟨hA, hB⟩ := hp.wf_tp.inv_sigma
+    have ⟨_, hA, hB⟩ := hp.wf_tp.inv_sigma
     WfTm.snd' hA hB hp
 
 theorem EqTm.cong_lam {Γ A A' B t t' l l'} :
@@ -316,14 +336,14 @@ theorem EqTm.lam_app {Γ A B f l l'} :
     Γ ⊢[max l l'] f : .pi l l' A B →
     Γ ⊢[max l l'] f ≡ .lam l l' A (.app l l' (B.subst (Expr.up Expr.wk)) (f.subst Expr.wk) (.bvar 0)) : .pi l l' A B :=
   fun hf =>
-    have ⟨hA, hB⟩ := hf.wf_tp.inv_pi
+    have ⟨_, hA, hB⟩ := hf.wf_tp.inv_pi
     EqTm.lam_app' hA hB hf
 
 theorem EqTm.pair_fst_snd {Γ A B p l l'} :
     Γ ⊢[max l l'] p : .sigma l l' A B →
     Γ ⊢[max l l'] p ≡ .pair l l' B (.fst l l' A B p) (.snd l l' A B p) : .sigma l l' A B :=
   fun hp =>
-    have ⟨hA, hB⟩ := hp.wf_tp.inv_sigma
+    have ⟨_, hA, hB⟩ := hp.wf_tp.inv_sigma
     EqTm.pair_fst_snd' hA hB hp
 
 theorem EqTm.symm_tm {Γ A t t' l} :
@@ -339,16 +359,30 @@ theorem EqTm.trans_tm {Γ A t t' t'' l} :
 
 /-! ## Term former inversion -/
 
-theorem WfTm.inv_lam {Γ A C b l l'} : Γ ⊢[max l l'] .lam l l' A b : C →
-    (Γ ⊢[l] A) ∧ ∃ B, ((A, l) :: Γ ⊢[l'] b : B) ∧ (Γ ⊢[max l l'] C ≡ .pi l l' A B) := by
+theorem WfTm.inv_bvar {Γ A i l} : Γ ⊢[l] .bvar i : A →
+  ∃ B, Lookup Γ i B l ∧ (Γ ⊢[l] A ≡ B) := by
+  suffices
+    (∀ {Γ}, WfCtx Γ → True) ∧
+    (∀ {Γ l A}, Γ ⊢[l] A → True) ∧
+    (∀ {Γ l A B}, Γ ⊢[l] A ≡ B → True) ∧
+    (∀ {Γ l t C}, Γ ⊢[l] t : C → ∀ {i}, t = .bvar i → ∃ B, Lookup Γ i B l ∧ (Γ ⊢[l] C ≡ B)) ∧
+    (∀ {Γ l t u A}, Γ ⊢[l] t ≡ u : A → True) from
+  fun h => this.2.2.2.1 h rfl
+  mutual_induction <;>
+    grind [EqTp.refl_tp, EqTp.symm_tp, EqTp.trans_tp, WfCtx.lookup_wf]
+
+theorem WfTm.inv_lam {Γ A C b l₀ l l'} : Γ ⊢[l₀] .lam l l' A b : C →
+    l₀ = max l l' ∧ (Γ ⊢[l] A) ∧
+      ∃ B, ((A, l) :: Γ ⊢[l'] b : B) ∧ (Γ ⊢[max l l'] C ≡ .pi l l' A B) := by
   suffices
       (∀ {Γ}, WfCtx Γ → True) ∧
       (∀ {Γ l A}, Γ ⊢[l] A → True) ∧
       (∀ {Γ l A B}, Γ ⊢[l] A ≡ B → True) ∧
-      (∀ {Γ l t C}, Γ ⊢[l] t : C → ∀ {A b l₁ l₂}, l = max l₁ l₂ → t = .lam l₁ l₂ A b →
-        (Γ ⊢[l₁] A) ∧ ∃ B, ((A, l₁) :: Γ ⊢[l₂] b : B) ∧ (Γ ⊢[max l₁ l₂] C ≡ .pi l₁ l₂ A B)) ∧
+      (∀ {Γ l t C}, Γ ⊢[l] t : C → ∀ {A b l₁ l₂}, t = .lam l₁ l₂ A b →
+        l = max l₁ l₂ ∧ (Γ ⊢[l₁] A) ∧
+          ∃ B, ((A, l₁) :: Γ ⊢[l₂] b : B) ∧ (Γ ⊢[max l₁ l₂] C ≡ .pi l₁ l₂ A B)) ∧
       (∀ {Γ l t u A}, Γ ⊢[l] t ≡ u : A → True) from
-    fun h => this.2.2.2.1 h rfl rfl
+    fun h => this.2.2.2.1 h rfl
   mutual_induction <;>
     grind [WfTp.pi, WfTm.wf_tp, EqTp.refl_tp, EqTp.symm_tp, EqTp.trans_tp]
 
@@ -370,3 +404,66 @@ theorem WfTm.inv_app {Γ B C f a l l'} : Γ ⊢[l'] .app l l' B f a : C →
     fun h => this.2.2.2.1 h rfl
   mutual_induction <;>
     grind [InvProof.tp_inst, WfTp.wf_ctx, EqTp.refl_tp, EqTp.symm_tp, EqTp.trans_tp]
+
+theorem WfTm.inv_pair {Γ B C t u l₀ l l'} : Γ ⊢[l₀] .pair l l' B t u : C →
+    l₀ = max l l' ∧ ∃ A,
+      (Γ ⊢[l] t : A) ∧
+      (Γ ⊢[l'] u : B.subst t.toSb) ∧
+      ((A, l) :: Γ ⊢[l'] B) ∧
+      (Γ ⊢[l₀] C ≡ .sigma l l' A B) := by
+  suffices
+    (∀ {Γ}, WfCtx Γ → True) ∧
+    (∀ {Γ l A}, Γ ⊢[l] A → True) ∧
+    (∀ {Γ l A B}, Γ ⊢[l] A ≡ B → True) ∧
+    (∀ {Γ l t C}, Γ ⊢[l] t : C → ∀ {B t' u' l₁ l₂}, t = .pair l₁ l₂ B t' u' →
+      l = max l₁ l₂ ∧ ∃ A,
+        (Γ ⊢[l₁] t' : A) ∧
+        (Γ ⊢[l₂] u' : B.subst t'.toSb) ∧
+        ((A, l₁) :: Γ ⊢[l₂] B) ∧
+        (Γ ⊢[l] C ≡ .sigma l₁ l₂ A B)) ∧
+    (∀ {Γ l t u A}, Γ ⊢[l] t ≡ u : A → True) from
+  fun h => this.2.2.2.1 h rfl
+  mutual_induction <;> grind [WfTp.sigma, WfTm.wf_tp, EqTp.refl_tp, EqTp.symm_tp, EqTp.trans_tp]
+
+theorem WfTm.inv_fst {Γ A B C p l₀ l l'} : Γ ⊢[l₀] .fst l l' A B p : C →
+    l₀ = l ∧ (Γ ⊢[max l l'] p : .sigma l l' A B) ∧ (Γ ⊢[l₀] C ≡ A) := by
+  suffices
+    (∀ {Γ}, WfCtx Γ → True) ∧
+    (∀ {Γ l A}, Γ ⊢[l] A → True) ∧
+    (∀ {Γ l A B}, Γ ⊢[l] A ≡ B → True) ∧
+    (∀ {Γ l t C}, Γ ⊢[l] t : C → ∀ {A B p l₁ l₂}, t = .fst l₁ l₂ A B p →
+    l = l₁ ∧ (Γ ⊢[max l₁ l₂] p : .sigma l₁ l₂ A B) ∧
+    (Γ ⊢[l] C ≡ A)) ∧
+    (∀ {Γ l t u A}, Γ ⊢[l] t ≡ u : A → True) from
+  fun h => this.2.2.2.1 h rfl
+  mutual_induction <;> grind [EqTp.refl_tp, EqTp.symm_tp, EqTp.trans_tp]
+
+theorem WfTm.inv_snd {Γ A B C p l₀ l l'} : Γ ⊢[l₀] .snd l l' A B p : C →
+    l₀ = l' ∧ (Γ ⊢[max l l'] p : .sigma l l' A B) ∧
+      (Γ ⊢[l₀] C ≡ B.subst (Expr.fst l l' A B p).toSb) := by
+  suffices
+    (∀ {Γ}, WfCtx Γ → True) ∧
+    (∀ {Γ l A}, Γ ⊢[l] A → True) ∧
+    (∀ {Γ l A B}, Γ ⊢[l] A ≡ B → True) ∧
+    (∀ {Γ l t C}, Γ ⊢[l] t : C → ∀ {A B p l₁ l₂}, t = .snd l₁ l₂ A B p →
+      l = l₂ ∧ (Γ ⊢[max l₁ l₂] p : .sigma l₁ l₂ A B) ∧
+      (Γ ⊢[l] C ≡ B.subst (Expr.fst l₁ l₂ A B p).toSb)) ∧
+      (∀ {Γ l t u A}, Γ ⊢[l] t ≡ u : A → True) from
+  fun h => this.2.2.2.1 h rfl
+  mutual_induction <;>
+    grind [InvProof.tp_inst, EqTp.refl_tp, EqTp.symm_tp, EqTp.trans_tp, WfTm.fst, WfTp.wf_ctx]
+
+theorem WfTm.inv_code {Γ A C l₀} : Γ ⊢[l₀] .code A : C →
+    ∃ l, l₀ = l+1 ∧ (Γ ⊢[l] A) ∧ (Γ ⊢[l+1] C ≡ .univ l) := by
+  suffices
+    (∀ {Γ}, WfCtx Γ → True) ∧
+    (∀ {Γ l A}, Γ ⊢[l] A → True) ∧
+    (∀ {Γ l A B}, Γ ⊢[l] A ≡ B → True) ∧
+    (∀ {Γ l t C}, Γ ⊢[l] t : C → ∀ {A}, t = .code A →
+      ∃ l₁, l = l₁+1 ∧ (Γ ⊢[l₁] A) ∧ (Γ ⊢[l₁+1] C ≡ .univ l₁)) ∧
+    (∀ {Γ l t u A}, Γ ⊢[l] t ≡ u : A → True) from
+  fun h => this.2.2.2.1 h rfl
+  mutual_induction <;> try grind [EqTp.refl_tp, WfTp.univ, WfTp.wf_ctx]
+  case conv ih _ _ eq =>
+    obtain ⟨_, rfl, _⟩ := ih eq
+    grind [EqTp.trans_tp, EqTp.symm_tp]
